---
title: Demo that Three Points Determine a Circle
---

Given the three points $$P_1 ( x_1 , y_1 )$$, $$P_2 ( x_2 , y_2 )$$, and $$P_3 ( x_3 , y_3 )$$,
how do we determine the circle?
The equation for a circle with its center at $$( a , b )$$ and radius $$r$$ is

$$
( x - a ) ^ 2 + ( y - b ) ^2 = r ^ 2 .
$$

Expanding this out, we have

$$
x ^ 2 + y ^ 2 - 2 a x - 2 b y + a ^2 + b ^ 2 - r ^ 2 = 0 ,
$$

which has the form

$$
\boxed{x ^ 2 + y ^ 2 + D x + E y + F = 0} \tag{1}
$$

where

$$
D = - 2 a , \quad E = - 2 b , \quad \text{and} \quad F = a^2 + b^2 - r^2 . \tag{2}
$$

Substituting the three points into eq. (1) gives the matrix equation

$$
\begin{bmatrix}
x_1 & y_1 & 1 \\
x_2 & y_2 & 1 \\
x_3 & y_3 & 1 \\
\end{bmatrix}
\begin{bmatrix}
D \\
E \\
F \\
\end{bmatrix} =
\begin{bmatrix}
- ( x_1 ^ 2 + y_1 ^ 2 ) \\
- ( x_2 ^ 2 + y_2 ^ 2 ) \\
- ( x_3 ^ 2 + y_3 ^ 2 ) \\
\end{bmatrix} .
$$

Let

$$
A = 
\begin{bmatrix}
x_1 & y_1 & 1 \\
x_2 & y_2 & 1 \\
x_3 & y_3 & 1 \\
\end{bmatrix} ,
$$

then Cramer's rule gives

$$
D = \frac{1}{\det{A}}
\det
\begin{bmatrix}
- ( x_1 ^ 2 + y_1 ^ 2 ) & y_1 & 1 \\
- ( x_2 ^ 2 + y_2 ^ 2 ) & y_2 & 1 \\
- ( x_3 ^ 2 + y_3 ^ 2 ) & y_3 & 1 \\
\end{bmatrix} ,
$$

$$
E = \frac{1}{\det{A}}
\det
\begin{bmatrix}
x_1 & - ( x_1 ^ 2 + y_1 ^ 2 ) & 1 \\
x_2 & - ( x_2 ^ 2 + y_2 ^ 2 ) & 1 \\
x_3 & - ( x_3 ^ 2 + y_3 ^ 2 ) & 1 \\
$$ ,

and

$$
F = \frac{1}{\det{A}}
\det
\begin{bmatrix}
x_1 & y_1 & - ( x_1 ^ 2 + y_1 ^ 2 ) \\
x_2 & y_2 & - ( x_2 ^ 2 + y_2 ^ 2 ) \\
x_3 & y_3 & - ( x_3 ^ 2 + y_3 ^ 2 ) \\
\end{bmatrix} .
$$

From eq. (2), the center and radius of the circle are then given by

$$
C ( a , b ) = C ( - D / 2, - E / 2 ) \quad \text{and} \quad r = \sqrt{ a^2 + b^2 - F} .
$$

[Demo](./circle.html)
